compiler/src/compiler/StringNameGen.v
@@ -4,13 +4,13 @@ Require Import compiler.NameGen.
 
 Local Open Scope string_scope.
 
-Axiom TODO: False.
+Axiom TODO_someone: False.
 
 Instance StringNameGen: NameGen string string. refine ({|
   freshNameGenState := fun l => "_x"; (* TODO this might clash with names in l *)
   genFresh s := (s, append s "'");
   allFreshVars s := fun x => (String.length s <= String.length x)
 |}).
-- case TODO.
-- case TODO.
+- case TODO_someone.
+- case TODO_someone.
 Defined.
